Challenge/Modexp/Submission/Proofs/Fast/FixedDirectStates.lean
@@ -18,55 +18,55 @@ abbrev outer := Exp.outer
 
 def otherWidth (s : State) (mem : ByteArray)
     (n bsize esize msize : Nat) : State :=
-  { s with pc := UInt256.ofNat 3660
+  { s with pc := UInt256.ofNat 3645
            stack := outer n bsize esize msize
            memory := mem }
 
 def checkThree (s : State) (mem : ByteArray)
     (n bsize esize msize : Nat) : State :=
-  { s with pc := UInt256.ofNat 3669
+  { s with pc := UInt256.ofNat 3654
            stack := outer n bsize esize msize
            memory := mem }
 
 def check65537 (s : State) (mem : ByteArray)
     (n bsize esize msize : Nat) : State :=
-  { s with pc := UInt256.ofNat 3690
+  { s with pc := UInt256.ofNat 3675
            stack := outer n bsize esize msize
            memory := mem }
 
 def special (s : State) (mem : ByteArray)
     (n bsize esize msize count : Nat) : State :=
-  { s with pc := UInt256.ofNat 3711
+  { s with pc := UInt256.ofNat 3696
            stack := UInt256.ofNat count :: outer n bsize esize msize
            memory := mem }
 
 def square (s : State) (mem : ByteArray)
     (n bsize esize msize count : Nat) : State :=
-  { s with pc := UInt256.ofNat 3712
+  { s with pc := UInt256.ofNat 3697
            stack := UInt256.ofNat count :: outer n bsize esize msize
            memory := mem }
 
 def squareReturn (s : State) (mem : ByteArray)
     (n bsize esize msize count : Nat) : State :=
-  { s with pc := UInt256.ofNat 3729
+  { s with pc := UInt256.ofNat 3714
            stack := UInt256.ofNat count :: outer n bsize esize msize
            memory := mem }
 
 def product (s : State) (mem : ByteArray)
     (n bsize esize msize : Nat) : State :=
-  { s with pc := UInt256.ofNat 3739
+  { s with pc := UInt256.ofNat 3724
            stack := UInt256.ofNat 0 :: outer n bsize esize msize
            memory := mem }
 
 def finish (s : State) (mem : ByteArray)
     (n bsize esize msize : Nat) : State :=
-  { s with pc := UInt256.ofNat 3756
+  { s with pc := UInt256.ofNat 3741
            stack := outer n bsize esize msize
            memory := mem }
 
 def fallback (s : State) (mem : ByteArray)
     (n bsize esize msize : Nat) : State :=
-  { s with pc := UInt256.ofNat 3761
+  { s with pc := UInt256.ofNat 3746
            stack := outer n bsize esize msize
            memory := mem }
 
